step-by-step tests

silveroak-opentitan/hmac/Spec/HMAC.v
@@ -16,6 +16,7 @@
 
 Require Import Coq.Lists.List.
 Require Import Coq.NArith.NArith.
+Require Import Cava.Util.BitArithmetic.
 Require Import HmacSpec.SHA256.
 Import ListNotations.
 Local Open Scope N_scope.
@@ -31,12 +32,9 @@ Local Open Scope N_scope.
    functions), and by L the byte-length of hash outputs (L=16 for MD5, L=20 for
    SHA-1).
  *)
-Definition B : nat := 64. (* block size for SHA-256 = 512 bits = 64 bytes *)
+Definition B : nat := 64. (* block size for SHA-256  = 512 bits = 64 bytes *)
 Definition L : nat := 32. (* output size for SHA-256 = 256 bits = 32 bytes *)
 
-(* TODO: move *)
-Definition concat_bytes (bs : list N) : N :=
-  fold_left (fun acc => N.lor (N.shiftl acc 8)) bs 0.
 
 (* From section 2:
 
@@ -94,6 +92,49 @@ Section HMAC_SHA256.
     H B ldata (N.lxor padded_key opad) inner.
 End HMAC_SHA256.
 
+
+(* Test 1 from https://csrc.nist.gov/CSRC/media/Projects/Cryptographic-Standards-and-Guidelines/documents/examples/HMAC_SHA256.pdf *)
+Definition data := 0x53616D706C65206D65737361676520666F72206B65796C656E3D626C6F636B6C656E.
+Definition K := 0x000102030405060708090A0B0C0D0E0F101112131415161718191A1B1C1D1E1F202122232425262728292A2B2C2D2E2F303132333435363738393A3B3C3D3E3F.
+Definition lK : nat := 64.
+Definition ldata : nat := 34.
+
+(* Check key padding *)
+Goal (padded_key lK K = K).
+Proof. vm_compute. reflexivity. Qed.
+
+(* Check K ^ ipad *)
+Goal (N.lxor (padded_key lK K) ipad
+     = 0x36373435323330313E3F3C3D3A3B383926272425222320212E2F2C2D2A2B282916171415121310111E1F1C1D1A1B181906070405020300010E0F0C0D0A0B0809).
+Proof. vm_compute. reflexivity. Qed.
+
+(* Check concatenation *)
+Goal (let lx := B in
+      let ly := ldata in
+      let x := N.lxor (padded_key lK K) ipad in
+      let y := data in
+      N.lor (N.shiftl x (N.of_nat (ly * 8))) y
+      = 0x36373435323330313E3F3C3D3A3B383926272425222320212E2F2C2D2A2B282916171415121310111E1F1C1D1A1B181906070405020300010E0F0C0D0A0B080953616D706C65206D65737361676520666F72206B65796C656E3D626C6F636B6C656E
+     ).
+Proof. vm_compute. reflexivity. Qed.
+
+(* Check inner hash result *)
+Goal (
+    H B ldata (N.lxor (padded_key lK K) ipad) data
+    = 0xC0918E14C43562B910DB4B8101CF8812C3DA2783C670BFF34D88B3B88E731716).
+Proof. vm_compute. reflexivity. Qed.
+
+(* Check final digest *)
+Goal (hmac_sha256 lK ldata K data
+      =0x8BB9A1DB9806F20DF7F77B82138C7914dD174D59E13DC4D0169C9057B133E1D62).
+Proof. vm_compute. reflexivity. Qed.
+
+
+(* Test case 1 from RFC 2104: *)
+Goal
+  (hmac_sha256 16 8 0x0b0b0b0b0b0b0b0b0b0b0b0b0b0b0b0b 0x4869205468657265
+   = 0x9294727a3638bb1c13f48ef8158bfc9d).
+Proof. Time vm_compute. reflexivity. Qed.
 (* Test case 1 from RFC 4231:
    https://datatracker.ietf.org/doc/html/rfc4231 *)
 Goal
