silveroak-opentitan/hmac/Spec/SHA256.v
@@ -158,7 +158,7 @@ Section WithMessage.
   (* N.B. FIPS is using a big-endian convention when splitting the 512 bits into
   32-bit blocks *)
   Definition M (j i : N) :=
-    let Mi := (padded_msg >> (512*i)) mod (2^512) in
+    let Mi := (padded_msg >> (512*(Nblocks-1-i))) mod (2^512) in
     (Mi >> (32*(15-j))) mod (2^32).
 
   (* From section 6.2.2 (step 1):
@@ -235,7 +235,117 @@ Section WithMessage.
     concat_digest H.
 End WithMessage.
 
-(* Test vector from https://csrc.nist.gov/CSRC/media/Projects/Cryptographic-Standards-and-Guidelines/documents/examples/SHA256.pdf *)
-Goal (let abc := ((97 << 16) | (98 << 8) | 99) in
+(**** Test vectors from
+      https://csrc.nist.gov/CSRC/media/Projects/Cryptographic-Standards-and-Guidelines/documents/examples/SHA256.pdf ****)
+
+Require Import Coq.Strings.Ascii.
+Require Import Coq.Strings.String.
+Require Import Cava.Util.BitArithmetic.
+
+Definition string_to_N (s : string) :=
+  concat_bytes (map N_of_ascii (list_ascii_of_string s)).
+
+Goal (let abc := string_to_N "abc" in
       sha256 24 abc = 0xba7816bf8f01cfea414140de5dae2223b00361a396177a9cb410ff61f20015ad).
 Proof. vm_compute. reflexivity. Qed.
+
+Section Test2.
+  Let msg_string := "abcdbcdecdefdefgefghfghighijhijkijkljklmklmnlmnomnopnopq"%string.
+  Let msg := string_to_N msg_string.
+  Let l := N.of_nat (String.length msg_string * 8).
+
+  (* Check message padding *)
+  Goal (padded_msg l msg
+        = 0x6162636462636465636465666465666765666768666768696768696A68696A6B696A6B6C6A6B6C6D6B6C6D6E6C6D6E6F6D6E6F706E6F70718000000000000000000000000000000000000000000000000000000000000000000000000000000000000000000000000000000000000000000000000000000000000000000001C0).
+  Proof. vm_compute. reflexivity. Qed.
+
+  (* Check first 16 blocks of W for first round (i=0):
+     W[0] = 61626364
+     W[1] = 62636465
+     W[2] = 63646566
+     W[3] = 64656667
+     W[4] = 65666768
+     W[5] = 66676869
+     W[6] = 6768696A
+     W[7] = 68696A6B
+     W[8] = 696A6B6C
+     W[9] = 6A6B6C6D
+     W[10] = 6B6C6D6E
+     W[11] = 6C6D6E6F
+     W[12] = 6D6E6F70
+     W[13] = 6E6F7071
+     W[14] = 80000000
+     W[15] = 00000000 *)
+  Goal (firstn 16 (W l msg 0) =
+        [ 0x61626364
+          ; 0x62636465
+          ; 0x63646566
+          ; 0x64656667
+          ; 0x65666768
+          ; 0x66676869
+          ; 0x6768696A
+          ; 0x68696A6B
+          ; 0x696A6B6C
+          ; 0x6A6B6C6D
+          ; 0x6B6C6D6E
+          ; 0x6C6D6E6F
+          ; 0x6D6E6F70
+          ; 0x6E6F7071
+          ; 0x80000000
+          ; 0x00000000]).
+  Proof. vm_compute. reflexivity. Qed.
+
+  (* Check W for second round (i=1):
+
+     W[0] = 00000000
+     W[1] = 00000000
+     W[2] = 00000000
+     W[3] = 00000000
+     W[4] = 00000000
+     W[5] = 00000000
+     W[6] = 00000000
+     W[7] = 00000000
+     W[8] = 00000000
+     W[9] = 00000000
+     W[10] = 00000000
+     W[11] = 00000000
+     W[12] = 00000000
+     W[13] = 00000000
+     W[14] = 00000000
+     W[15] = 000001C0 *)
+  Goal (firstn 16 (W l msg 1) =
+        [ 0x00000000
+          ; 0x00000000
+          ; 0x00000000
+          ; 0x00000000
+          ; 0x00000000
+          ; 0x00000000
+          ; 0x00000000
+          ; 0x00000000
+          ; 0x00000000
+          ; 0x00000000
+          ; 0x00000000
+          ; 0x00000000
+          ; 0x00000000
+          ; 0x00000000
+          ; 0x00000000
+          ; 0x000001C0 ]).
+  Proof. vm_compute. reflexivity. Qed.
+
+  (* Check digest after first round *)
+  Goal (sha256_step l msg H0 0
+        = [ 0x85E655D6
+            ; 0x417A1795
+            ; 0x3363376A
+            ; 0x624CDE5C
+            ; 0x76E09589
+            ; 0xCAC5F811
+            ; 0xCC4B32C1
+            ; 0xF20E533A ]).
+  Proof. vm_compute. reflexivity. Qed.
+
+  (* Check final digest *)
+  Goal (sha256 l msg
+        = 0x248D6A61D20638B8E5C026930C3E6039A33CE45964FF2167F6ECEDD419DB06C1).
+  Proof. vm_compute. reflexivity. Qed.
+End Test2.
